\section*{Problem 1.}
\subsection*{Question}
Using the second quantized formalism show that for non-interacting fermions

\begin{equation*}
\Omega_{0}^{F}
=
- k_{B} T \sum_{i} \ln \left( 1 + e^{-\beta \left( \epsilon_{i} - \mu \right)} \right)
\end{equation*}
where $\epsilon_{i}$ denotes the $i$-th one-particle level.

\subsection*{Solution}
On the lecture using the second quantization we derived, that for non-interacting bosons the grand-canonical potential is

\begin{equation} \label{eq:1}
\Omega_{0}^{B}
=
k_{B} T \sum_{i} \ln \left( 1 - e^{-\beta \left( \epsilon_{i} - \mu \right)} \right)
\end{equation}
We know, that the grand-canonical partition function at fixed $T$ and $\mu$ is

\begin{equation} \label{eq:2}
Z_{0}
=
e^{-\beta \Omega_{0}^{F,B}}
=
Tr \left( e^{-\beta \hat{K}_{0}} \right)
\end{equation}
where

\begin{equation} \label{eq:3}
\hat{K}_{0}
=
\hat{H} - \mu \hat{N}
\equiv
\sum_{k,s} \left( \epsilon_{k} - \mu \right) a_{k,s}^{\dagger} a_{k,s}
\end{equation}
Here, $\epsilon_{k}$ is the 1 particle kinetic energy of the $k$-th particle and the Hamiltonian $\hat{H} = \sum_{k,s} \epsilon_{k} a_{k,s}^{\dagger} a_{k,s}$. We can expand equation (\ref{eq:2}) in the second quantization in the following way:

\begin{equation} \label{eq:4}
Z_{0}
=
\sum_{n_{1}} \sum_{n_{2}} \dots
\Braket{n_{1}, n_{2} \dots|e^{-\beta \sum_{k,s} \left( \epsilon_{k} - \mu \right) a_{k,s}^{\dagger} a_{k,s}}|n_{1}, n_{2} \dots}
\end{equation}
The operator inside the sandwich could be expanded into the product

\begin{equation} \label{eq:5}
e^{-\beta \sum_{k,s} \left( \epsilon_{k} - \mu \right) a_{k,s}^{\dagger} a_{k,s}}
=
e^{-\beta \left( \epsilon_{1} - \mu \right) a_{1}^{\dagger} a_{1}}
*
e^{-\beta \left( \epsilon_{2} - \mu \right) a_{2}^{\dagger} a_{2}}
*
\dots
\ .
\end{equation}
Using this, the equation (\ref{eq:4}) could be further expanded into another product:

\begin{equation} \label{eq:6}
Z_{0}
=
\left( \sum_{n_{1}\ =\ 0}^{\infty} \Braket{n_{1}|e^{-\beta \left( \epsilon_{1} - \mu \right) a_{1}^{\dagger} a_{1}}|n_{1}} \right)
*
\left( \sum_{n_{2}\ =\ 0}^{\infty} \Braket{n_{2}|e^{-\beta \left( \epsilon_{2} - \mu \right) a_{2}^{\dagger} a_{2}}|n_{2}} \right)
*
\dots
\end{equation}
Since $a^{\dagger}_{k} a_{k} = n_{k}$, therefore the exponents could be rewritten in the following form:
\begin{equation} \label{eq:7}
Z_{0}
=
\left( \sum_{n_{1}\ =\ 0}^{\infty} \Braket{n_{1}|e^{-\beta \left( \epsilon_{1} - \mu \right) n_{1}}|n_{1}} \right)
*
\left( \sum_{n_{2}\ =\ 0}^{\infty} \Braket{n_{2}|e^{-\beta \left( \epsilon_{2} - \mu \right) n_{2}}|n_{2}} \right)
*
\dots
\end{equation}
The operators could be multiply out from the sandwiches:

\begin{equation} \label{eq:8}
\Braket{n_{k}|e^{-\beta \left( \epsilon_{k} - \mu \right) n_{k}}|n_{k}}
=
e^{-\beta \left( \epsilon_{k} - \mu \right) n_{k}} \underbrace{\Braket{n_{k}|n_{k}}}_{=1}
\end{equation}
Thus equation (\ref{eq:7}) could be rewritten into the form of a product of sum of exponentials

\begin{equation} \label{eq:9}
Z_{0}
=
\prod_{k\ =\ 1}^{\infty}
\left(
\sum_{n_{k}\ =\ 0}^{\infty} e^{-\beta \left( \epsilon_{k} - \mu \right) n_{k}}
\right)
\ .
\end{equation}
The $n_{k}$ occupation number can take the following values:

\begin{equation*}
n_{k}
=
\begin{cases}
0,1 & \text{for fermions} \\
0,1,2,\dots & \text{for bosons}
\end{cases}
\end{equation*}
Since our task is to derive the $\Omega_{0}$ for fermions, we use the first fermionic case here, $n_{k} \in \left\{ 0,1 \right\}$. With this, the equation (\ref{eq:9}) could be rephrased in the following way:

\begin{equation} \label{eq:10}
Z_{0}
=
\prod_{k\ =\ 1}^{\infty}
\left(
\sum_{n_{k}\ =\ 0}^{1} e^{-\beta \left( \epsilon_{k} - \mu \right) n_{k}}
\right)
=
\prod_{k\ =\ 1}^{\infty}
\left(
e^{-\beta \left( \epsilon_{k} - \mu \right) * 0}
+
e^{-\beta \left( \epsilon_{k} - \mu \right) * 1}
\right)
=
\prod_{k\ =\ 1}^{\infty}
\left(
1
+
e^{-\beta \left( \epsilon_{k} - \mu \right)}
\right)
\end{equation}
Substituting back to equation (\ref{eq:2}), $\Omega_{0}^{F,B}$ could be expressed with

\begin{equation} \label{eq:11}
\Omega_{0}^{F,B}
=
- \frac{1}{\beta} \ln \left( Z_{0} \right)
\end{equation}
\begin{equation} \label{eq:12}
\Omega_{0}^{F}
=
-k_{B} T \ln \left(
\prod_{k\ =\ 1}^{\infty}
\left(
1
+
e^{-\beta \left( \epsilon_{k} - \mu \right)}
\right)
\right)
=
-k_{B} T \sum_{k\ =\ 0}^{\infty} \ln \left( 1 + e^{-\beta \left( \epsilon_{k} - \mu \right)} \right)
\end{equation}
Thus we've reached to our goal.