\subsection*{Graph 3. \coord}

\begin{center}
\begin{tikzpicture}
  \begin{feynman}
    \vertex[empty dot, label=below:{$X$}] (a1){};
    \vertex[dot, right=1.5cm of a1, label=above:{$X_{2}'$}] (a2){};
    \vertex[dot, right=1.5cm of a2, label=above:{$X_{2}$}] (a3){};
    \vertex[dot, right=1.5cm of a3, label=below:{$X_{1}$}] (a4){};
    \vertex[empty dot, right=1.5cm of a4, label=below:{$X'$}] (a5){};
    
    \vertex[dot, above=1.5cm of a4, label=below right:{$X_{1}'$}] (b1){};
    
    \vertex[above=0.75cm of b1] (c1);
    \vertex[right=0.75cm of a2] (c2);

    \diagram* {
      {[edges=fermion]
        (a5) -- (a4) -- (a3) -- (a2) -- (a1),
      },
      (a4) -- [dash pattern=on 4pt off 4pt] (b1),

    };
    \centerarc[fermion](c1)(0:360:0.75)
    \centerarc[dash pattern=on 4pt off 4pt](c2)(180:360:0.75)

  \end{feynman}
\end{tikzpicture}
\end{center}

\subsection*{Solution}
Fermion propagator lines are building connections between the points $\left( X' \to X_{1} \right)$, $\left( X_{2}' \to X \right)$, $\left( X_{1} \to X_{2} \right)$, $\left( X_{2} \to X_{2}' \right)$ and $\left( X_{1}' \to X_{1}' \right)$, where the last one is a fermion loop. Their contributions are:

\begin{align} \label{eq:19}
- \mathcal{G}_{0} \left( X_{i}, X_{j} \right)
&\to
\left[ - \mathcal{G}_{0} \left( X_{2}, X_{1} \right) \right]
*
\left[ - \mathcal{G}_{0} \left( X_{2}', X_{2} \right) \right]
*
\left[ - \mathcal{G}_{0} \left( X_{1}', X_{1}' \right) \right]
*
\left[ - \mathcal{G}_{0} \left( X_{1}, X' \right) \right]
*
\left[ - \mathcal{G}_{0} \left( X, X_{2}' \right) \right]
= \nonumber \\
&=
- \mathcal{G}_{0} \left( X_{2}, X_{1} \right)
*
\mathcal{G}_{0} \left( X_{2}', X_{2} \right)
*
\mathcal{G}_{0} \left( X_{1}', X_{1}' \right)
*
\mathcal{G}_{0} \left( X_{1}, X' \right)
*
\mathcal{G}_{0} \left( X, X_{2}' \right)
\end{align}
Fermion loops also contribute to the Green's function. Since there are only one of them its contribution is

\begin{equation} \label{eq:20}
\left( -1 \right)^{F} \to \left( -1 \right)^{1} = -1
\end{equation}
Interaction happens between $\left( X_{1}, X_{1}' \right)$ and $\left( X_{2}, X_{2}' \right)$. Their contributions are

\begin{equation} \label{eq:21}
- \frac{1}{\hbar} v \left( X_{i} X_{i}' \right)
\to
\left( - \frac{1}{\hbar} \right) v \left( X_{1} X_{1}' \right)
*
\left( - \frac{1}{\hbar} \right) v \left( X_{2} X_{2}' \right)
=
\frac{1}{\hbar^{2}} v \left( X_{1} X_{1}' \right) v \left( X_{2} X_{2}' \right)
\end{equation}
Putting them all together, we need to integrate over all the internal $X_{i}$ points to get the Green's function:

\begin{align} \label{eq:22}
\mathcal{G} \left( X, X' \right)
&=
\int \text{d}X_{1} \int \text{d}X_{2} \int \text{d}X_{1}' \int \text{d}X_{2}'
*
\left( -1 \right)
*
\frac{1}{\hbar^{2}} v \left( X_{1} X_{1}' \right) v \left( X_{2} X_{2}' \right)
\times \nonumber \\
&\times
\left[
- \mathcal{G}_{0} \left( X_{2}, X_{1} \right)
*
\mathcal{G}_{0} \left( X_{2}', X_{2} \right)
*
\mathcal{G}_{0} \left( X_{1}', X_{1}' \right)
*
\mathcal{G}_{0} \left( X_{1}, X' \right)
*
\mathcal{G}_{0} \left( X, X_{2}' \right)
\right]
\end{align}
Where the $(-1)$ term cancels out the minus sign at the $\mathcal{G}_{0}$ contributions. Thus the Green's function is the following:

\begin{align} \label{eq:23}
\mathcal{G} \left( X, X' \right)
&=
\int \text{d}X_{1} \int \text{d}X_{2} \int \text{d}X_{1}' \int \text{d}X_{2}'
*
\frac{1}{\hbar^{2}} v \left( X_{1} X_{1}' \right) v \left( X_{2} X_{2}' \right)
\times \nonumber \\
&\times
\mathcal{G}_{0} \left( X_{2}, X_{1} \right)
*
\mathcal{G}_{0} \left( X_{2}', X_{2} \right)
*
\mathcal{G}_{0} \left( X_{1}', X_{1}' \right)
*
\mathcal{G}_{0} \left( X_{1}, X' \right)
*
\mathcal{G}_{0} \left( X, X_{2}' \right)
\end{align}