\subsection*{Graph 10. \coord}

\begin{center}
\begin{tikzpicture}
  \begin{feynman}
    \vertex[empty dot, label=below:{$X$}] (a1){};
    \vertex[dot, right=1.5cm of a1, label=above:{$X_{1}'$}] (a2){};
    \vertex[dot, right=1.5cm of a2, label=below:{$X_{2}'$}] (a3){};
    \vertex[dot, right=1.5cm of a3, label=above:{$X_{1}$}] (a4){};
    \vertex[dot, right=1.5cm of a4, label=below:{$X_{2}$}] (a5){};
    \vertex[empty dot, right=1.5cm of a5, label=below:{$X'$}] (a6){};

    \diagram* {
      {[edges=fermion]
        (a6) -- (a5) -- (a4) -- (a3) -- (a2) -- (a1),
      },
    };
    \draw[dash pattern=on 4pt off 4pt, bend right=90] (a5) to (a3);
    \draw[dash pattern=on 4pt off 4pt, bend left=90] (a4) to (a2);
    %\centerarc[dash pattern=on 4pt off 4pt](a3)(180:360:1.5)
    %\centerarc[dash pattern=on 4pt off 4pt](a4)(0:180:1.5)

  \end{feynman}
\end{tikzpicture}
\end{center}

\subsection*{Solution}
Fermion propagator lines are building connections between the points $\left( X' \to X_{2} \right)$, $\left( X_{2} \to X_{1} \right)$, $\left( X_{1} \to X_{2}' \right)$, $\left( X_{2}' \to X_{1}' \right)$ and $\left( X_{1}' \to X \right)$. Their contributions are:

\begin{align} \label{eq:60}
- \mathcal{G}_{0} \left( X_{i}, X_{j} \right)
&\to
\left[ - \mathcal{G}_{0} \left( X_{2}, X' \right) \right]
*
\left[ - \mathcal{G}_{0} \left( X_{1}, X_{2} \right) \right]
*
\left[ - \mathcal{G}_{0} \left( X_{2}', X_{1} \right) \right]
*
\left[ - \mathcal{G}_{0} \left( X_{1}', X_{2}' \right) \right]
*
\left[ - \mathcal{G}_{0} \left( X, X_{1}' \right) \right]
= \nonumber \\
&=
- \mathcal{G}_{0} \left( X_{2}, X' \right)
*
\mathcal{G}_{0} \left( X_{1}, X_{2} \right)
*
\mathcal{G}_{0} \left( X_{2}', X_{1} \right)
*
\mathcal{G}_{0} \left( X_{1}', X_{2}' \right)
*
\mathcal{G}_{0} \left( X, X_{1}' \right)
\end{align}
Interaction happens between $\left( X_{1}, X_{1}' \right)$ and $\left( X_{2}, X_{2}' \right)$. Their contributions are

\begin{equation} \label{eq:61}
- \frac{1}{\hbar} v \left( X_{i} X_{i}' \right)
\to
\left( - \frac{1}{\hbar} \right) v \left( X_{1} X_{1}' \right)
*
\left( - \frac{1}{\hbar} \right) v \left( X_{2} X_{2}' \right)
=
\frac{1}{\hbar^{2}} v \left( X_{1} X_{1}' \right) v \left( X_{2} X_{2}' \right)
\end{equation}
Putting them all together, we need to integrate over all the internal $X_{i}$ points to get the final form for the integral of the Green's function:

\begin{align} \label{eq:62}
\mathcal{G} \left( X, X' \right)
&=
\int \text{d}X_{1} \int \text{d}X_{2} \int \text{d}X_{1}' \int \text{d}X_{2}'
*
\frac{1}{\hbar^{2}} v \left( X_{1} X_{1}' \right) v \left( X_{2} X_{2}' \right)
\times \nonumber \\
&\times
\left[
- \mathcal{G}_{0} \left( X_{2}, X' \right)
*
\mathcal{G}_{0} \left( X_{1}, X_{2} \right)
*
\mathcal{G}_{0} \left( X_{2}', X_{1} \right)
*
\mathcal{G}_{0} \left( X_{1}', X_{2}' \right)
*
\mathcal{G}_{0} \left( X, X_{1}' \right)
\right]
\end{align}